src/HolSmt/Z3_ProofReplay.sml
@@ -29,6 +29,11 @@ struct
   val IMP_DISJ_2 = HolSmtTheory.IMP_DISJ_2
   val IMP_FALSE = HolSmtTheory.IMP_FALSE
 
+  val update_ss = simpLib.&& (simpLib.++ (intSimps.int_ss,
+      simpLib.std_conv_ss {name = "word_EQ_CONV", pats = [``(x :'a word) = y``],
+        conv = wordsLib.word_EQ_CONV}),
+    [combinTheory.UPDATE_def, boolTheory.EQ_SYM_EQ])
+
   fun check_proof prf =
   let
     val _ = if !SolverSpec.trace > 1 then
@@ -687,8 +692,7 @@ struct
         handle Feedback.HOL_ERR _ =>
 
         (*Profile.profile "rewrite(update)"*) (fn () =>
-          simpLib.SIMP_PROVE intSimps.int_ss [combinTheory.UPDATE_def,
-            boolTheory.EQ_SYM_EQ] t) ()
+          simpLib.SIMP_PROVE update_ss [] t) ()
         handle Feedback.HOL_ERR _ =>
 
         (*Profile.profile "rewrite(cache)"*) (fn () =>
@@ -699,6 +703,23 @@ struct
                 (*Profile.profile "rewrite(REAL_ARITH)"*) realLib.REAL_ARITH t
               else
                 (*Profile.profile "rewrite(ARITH_PROVE)"*) intLib.ARITH_PROVE t
+            handle Feedback.HOL_ERR _ =>
+
+              (*TODO*) Profile.profile "rewrite(WORD_ARITH_CONV)" (fn () =>
+              Drule.EQT_ELIM (wordsLib.WORD_ARITH_CONV t)
+                handle Conv.UNCHANGED =>
+                  raise (Feedback.mk_HOL_ERR "" "" "")) ()
+            handle Feedback.HOL_ERR _ =>
+
+              (*TODO*) Profile.profile "rewrite(WORD_BIT_EQ)" (fn () =>
+              Drule.EQT_ELIM (Conv.THENC (simpLib.SIMP_CONV (simpLib.++
+                (simpLib.++ (bossLib.std_ss, wordsLib.WORD_ss),
+                wordsLib.WORD_BIT_EQ_ss)) [],
+                tautLib.TAUT_CONV) t)) ()
+            handle Feedback.HOL_ERR _ =>
+
+              (*TODO*) Profile.profile "rewrite(WORD_DECIDE)"
+                wordsLib.WORD_DECIDE t
             handle Feedback.HOL_ERR _ =>
 
               (*TODO*) Profile.profile "rewrite(WORD_DP)" (fn () =>
@@ -793,6 +814,10 @@ struct
         Drule.LIST_MP thms (Z3_ProformaThms.prove (!theorem_cache) concl)
         handle Feedback.HOL_ERR _ =>
 
+        (*Profile.profile "th_lemma(update)"*) (fn () => Drule.LIST_MP thms 
+          (simpLib.SIMP_PROVE update_ss [] concl)) ()
+        handle Feedback.HOL_ERR _ =>
+
         let val (dict, concl) = generalize_ite concl
             val th = if term_contains_real_ty concl then
                 (*Profile.profile "th_lemma(REAL_ARITH)"*)
@@ -800,6 +825,23 @@ struct
               else
                 (*Profile.profile "th_lemma(ARITH_PROVE)"*)
                   intLib.ARITH_PROVE concl
+            handle Feedback.HOL_ERR _ =>
+
+              (*TODO*) Profile.profile "th_lemma(WORD_ARITH_CONV)" (fn () =>
+              Drule.EQT_ELIM (wordsLib.WORD_ARITH_CONV concl)
+                handle Conv.UNCHANGED =>
+                  raise (Feedback.mk_HOL_ERR "" "" "")) ()
+            handle Feedback.HOL_ERR _ =>
+
+              (*TODO*) Profile.profile "th_lemma(WORD_BIT_EQ)" (fn () =>
+              Drule.EQT_ELIM (Conv.THENC (simpLib.SIMP_CONV (simpLib.++
+                (simpLib.++ (bossLib.std_ss, wordsLib.WORD_ss),
+                wordsLib.WORD_BIT_EQ_ss)) [],
+                tautLib.TAUT_CONV) concl)) ()
+            handle Feedback.HOL_ERR _ =>
+
+              (*TODO*) Profile.profile "th_lemma(WORD_DECIDE)"
+                wordsLib.WORD_DECIDE concl
             handle Feedback.HOL_ERR _ =>
 
               (*TODO*) Profile.profile "th_lemma(WORD_DP)" (fn () =>
