examples/lambda/barendregt/reductionEval.sml
@@ -89,7 +89,7 @@ end
 fun bsrw_ss() = betafy(srw_ss())
 
 val {export = export_betarwt,...} = ThmSetData.new_exporter "betasimp" add_rwts
-
+fun bstore_thm (trip as (n,t,tac)) = store_thm trip before export_betarwt n
 
 (* ----------------------------------------------------------------------
     A reducer for weak head reduction.
